verif/verif_movetokey.v
@@ -1,0 +1,160 @@
+(** * verif_movetokey.v : Correctness proof of moveToKey *)
+
+Require Import VST.floyd.proofauto.
+Require Import VST.floyd.library.
+Require Import relation_mem.
+Instance CompSpecs : compspecs. make_compspecs prog. Defined.
+Definition Vprog : varspecs. mk_varspecs prog. Defined.
+
+Require Import VST.msl.wand_frame.
+Require Import VST.msl.iter_sepcon.
+Require Import VST.floyd.reassoc_seq.
+Require Import VST.floyd.field_at_wand.
+Require Import FunInd.
+Require Import btrees.
+Require Import btrees_sep.
+Require Import btrees_spec.
+Require Import index.
+Require Import verif_findindex.
+
+Lemma Zsuccminusone: forall x,
+    (Z.succ x) -1 = x.
+Proof. intros. rep_omega. Qed.
+
+Lemma body_moveToKey: semax_body Vprog Gprog f_moveToKey moveToKey_spec.
+Proof.
+  start_function.
+  destruct r as [[[root numRec] depth] prel].
+  pose (r:=(root,numRec,depth,prel)). fold r.
+  destruct n as [ptr0 le isLeaf First Last xn].
+  pose (n:=btnode val ptr0 le isLeaf First Last xn). fold n.
+  unfold cursor_rep. Intros anc_end. Intros idx_end. unfold r.
+  forward.                      (* cursor->ancestors[level]=node *)
+  { unfold partial_cursor_wf in H0. entailer!. destruct H0.
+    (* TODO: rep_omega should work here? *)
+    split. omega. rewrite MTD_eq in H1. simpl in H1. auto. }
+  forward.                      (* cursor->level = level *)
+  gather_SEP 1 2 3 4 5.         (* the cursor, we a new node *)
+  assert(subnode n root).
+  { unfold get_root in H. simpl in H. fold n in H. apply cursor_subnode in H. auto. }
+  apply subnode_rep with (proot:=getval root) in H3.
+  unfold relation_rep. Intros proot. rewrite btnode_rep_getval. Intros. subst proot.
+  rewrite H3. simpl in H1. subst xn. Intros xn. rewrite btnode_rep_getval. Intros. subst.
+  normalize.
+  assert (getval n = pn). unfold n. simpl. auto. rewrite H1.
+  unfold n.
+  (* for some reason, unfold_btnode_rep at 1 takes a long time here *)
+  replace_SEP 6 (malloc_token Tsh tbtnode pn *
+  field_at Tsh tbtnode (DOT _numKeys) (Vint(Int.repr (Z.of_nat (numKeys n)))) pn *
+  field_at Tsh tbtnode (DOT _isLeaf) (Val.of_bool isLeaf) pn *
+  field_at Tsh tbtnode (DOT _FirstLeaf) (Val.of_bool First) pn *
+  field_at Tsh tbtnode (DOT _LastLeaf) (Val.of_bool Last) pn *
+  match ptr0 with
+  | None => field_at Tsh tbtnode (DOT _ptr0) nullval pn
+  | Some n' => match n' with btnode _ _ _ _ _ p' => field_at Tsh tbtnode (DOT _ptr0) p' pn * btnode_rep n' p' end end *
+  field_at Tsh tbtnode (DOT _entries) (le_to_list_complete le) pn *
+  le_iter_sepcon le).
+  entailer!. apply derives_refl.
+  Intros.
+  forward.                      (* t'3=node->isLeaf *)
+  { entailer!. destruct isLeaf; simpl; auto. }
+  forward_if.
+  - forward_call (n,key,pn).    (* t'1=findRecordIndex(node,key) *)
+    + admit.
+    + simpl. entailer!. admit.  (* what is this goal? *)
+    + rewrite unfold_btnode_rep with (n:=n) (p:=pn). unfold n.
+      rewrite prop_true_andp by auto. cancel.
+      change_compspecs CompSpecs. cancel.
+    + unfold n. simpl. rewrite H4. auto.
+    + forward.                  (* cursor->ancestorsIdx[level]=t'1 *)
+      { entailer!. clear -H0. unfold partial_cursor_wf in H0. destruct H0.
+        split. omega. rewrite MTD_eq in H0. simpl in H0. auto. }
+      gather_SEP 0 7.
+      replace_SEP 0 (btnode_rep root (getval root)).
+      entailer!. apply wand_frame_elim.
+      gather_SEP 0 6 7 8 9.
+      replace_SEP 0 (relation_rep r pr).
+      entailer!. Exists (getval root). cancel. apply derives_refl.
+      forward.                  (* return *)
+      Exists (getval root). entailer!.
+      unfold cursor_rep.
+      Exists (sublist 1 (Zlength anc_end) anc_end). Exists (sublist 1 (Zlength idx_end) idx_end).
+      cancel.
+      pose (ii:=findRecordIndex' le key (ip 0)). fold ii.
+      assert(moveToKey val (btnode val ptr0 le true First Last pn) key c (length c) = (n,ii)::c).
+      (* this should be true *) admit.
+      rewrite H24. rewrite Zlength_cons.
+      rewrite Zsuccminusone. autorewrite with sublist. rewrite upd_Znth0. rewrite upd_Znth0. simpl.
+      rewrite <- app_assoc. rewrite <- app_assoc. simpl. cancel.
+      apply derives_refl.
+  - forward_call(n,key,pn).     (* t'2=findChildIndex(node,key) *)
+    + admit.
+    + simpl. entailer!.
+      destruct (pTree_from_elements).
+      admit.                    (* THIS IS FALSE *)
+      admit.
+    + rewrite unfold_btnode_rep with (n:=n) (p:=pn). unfold n. rewrite prop_true_andp by auto.
+      cancel. change_compspecs CompSpecs. cancel.
+    + unfold n. simpl. rewrite H4. auto.
+    + forward.                  (* cursor->ancestors[level]=i *)
+      { entailer!. clear -H0. unfold partial_cursor_wf in H0. destruct H0. split. omega.
+        rewrite MTD_eq in H0. simpl in H0. auto. }
+      pose (i:=findChildIndex n key). fold i.
+      gather_SEP 1 2 3 4 5.
+      replace_SEP 0 (cursor_rep ((n,i)::c) r pc).
+      entailer!. unfold cursor_rep. unfold r.
+      Exists (sublist 1 (Zlength anc_end) anc_end). Exists (sublist 1 (Zlength idx_end) idx_end).
+      entailer!. autorewrite with sublist. rewrite upd_Znth0. rewrite upd_Znth0. simpl.
+      rewrite <- app_assoc. rewrite <- app_assoc. simpl. rewrite Zsuccminusone.
+      cancel. apply derives_refl.
+      (* gather_SEP 1 3. *)
+      (* replace_SEP 0 (btnode_rep root (getval root)). *)
+      (* entailer!. apply wand_frame_elim. *)
+      (* gather_SEP 0 2 3 4 5. *)
+      (* replace_SEP 0 (relation_rep r pr). *)
+      (* entailer!. Exists (getval root). cancel. apply derives_refl. *)
+      forward_if ( EX pchild:val, EX child:node val, PROP (pchild=getval child; nth_node i n = Some child)
+     LOCAL (temp _i (rep_index i); temp _t'3 (Val.of_bool isLeaf); temp _cursor pc; 
+     temp _node pn; temp _level (Vint (Int.repr (Zlength c))); temp _child pchild)
+     SEP (cursor_rep ((n, i) :: c) r pc; btnode_rep n pn;
+     field_at Tsh trelation [StructField _root] (getval root) pr;
+     btnode_rep (btnode val ptr0 le isLeaf First Last pn) pn -* btnode_rep root (getval root);
+     field_at Tsh trelation [StructField _numRecords] (Vint (Int.repr (Z.of_nat numRec))) pr;
+     field_at Tsh trelation [StructField _depth] (Vint (Int.repr (Z.of_nat depth))) pr;
+     malloc_token Tsh trelation pr))%assert.
+      * rewrite unfold_btnode_rep. unfold n. Intros.
+        destruct ptr0 eqn:HPTR0.
+        destruct n0 as [ptr00 le0 isLeaf0 F0 L0 x0]. Intros.
+        forward.                (* child=node->ptr0 *)
+        Exists x0. Exists (btnode val ptr00 le0 isLeaf0 F0 L0 x0).
+        entailer!.
+        destruct i eqn:HI. auto.
+        (* contradiction in H5 *) admit.
+        fold n. apply derives_refl.
+        (* ptr0 can't be none if isLeaf is false *)
+        admit.
+      * rewrite unfold_btnode_rep. unfold n. Intros.
+        (* I need to show that entries[i] is rep somewhere *)
+        (* forward.               (* child=node->entries+i.ptr.child *) *)
+        admit.
+      * Intros pchild. Intros child.
+        gather_SEP 1 3.
+        replace_SEP 0 (btnode_rep root (getval root)).
+        entailer!. apply wand_frame_elim.
+        gather_SEP 0 2 3 4 5.
+        replace_SEP 0 (relation_rep r pr).
+        entailer!. Exists (getval root). cancel. apply derives_refl.
+        { forward_call(child,key,pchild,(n,i)::c,pc,r,pr).
+          - admit.              (* cursor length *)
+          - admit.              (* false *)
+          - admit.              (* false *)
+          - split3.
+            + simpl. split. auto. destruct i. unfold n in H6. simpl in H6. auto. auto.
+            + unfold partial_cursor_wf. admit. (* cursor length *)
+            + split; auto.
+          - forward.            (* return *)
+            Exists p'. entailer!.
+            assert((moveToKey val child key ((n, i) :: c) (S (length c))) =  (moveToKey val (btnode val ptr0 le false First Last pn) key c (length c))).
+            admit.
+            rewrite H14. apply derives_refl. }
+Admitted.
